removing bench; adding get_mem_region correct proof; starting check_mem_aux

clight/interpreter.h
@@ -40,10 +40,10 @@ struct bpf_state {
   int state_pc;
   int bpf_flag;
   unsigned long long regsmap[11];
-  unsigned int mrs_num;
-  struct memory_region *mrs;
   int ins_len;
   const unsigned long long * ins;
+  unsigned int mrs_num;
+  struct memory_region *mrs;
 };
 
 unsigned long long bpf_interpreter(struct bpf_state *, unsigned int);
