model/Syntax.v
@@ -1,9 +1,21 @@
 From compcert Require Import Ctypes AST Integers.
 
-From bpf.comm Require Import Int16 Regs.
+From bpf.comm Require Import Int16 Regs rBPFAST.
 
 (** For use to distinguish ALU32 and ALU64 *)
 Inductive arch := A32 | A64.
+
+Lemma arch_eq: forall (x y: arch), {x=y} + {x<>y}.
+Proof.
+  decide equality.
+Defined.
+
+Definition arch_eqb (a0 a1: arch) : bool :=
+  match a0, a1 with
+  | A32, A32
+  | A64, A64 => true
+  | _, _ => false
+  end.
 
 (** For condition flags *)
 (*Inductive signedness := Signed | Unsigned.*)
@@ -18,6 +30,35 @@ Inductive cond :=
 | Ne
 .
 
+Lemma signedness_eq32: forall (s1 s2: signedness), {s1=s2} + {s1<>s2}.
+Proof.
+  decide equality.
+Defined.
+
+Definition signedness_eqb (s1 s2: signedness) :=
+  match s1, s2 with
+  | Signed, Signed
+  | Unsigned, Unsigned => true
+  | _, _ => false
+  end.
+
+Lemma cond_eq: forall (x y: cond), {x=y} + {x<>y}.
+Proof.
+  decide equality. all: apply signedness_eq32.
+Defined.
+
+Definition cond_eqb (c0 c1: cond): bool :=
+  match c0, c1 with
+  | Eq, Eq
+  | SEt, SEt
+  | Ne, Ne => true
+  | Gt s0, Gt s1
+  | Ge s0, Ge s1
+  | Lt s0, Lt s1
+  | Le s0, Le s1 => signedness_eqb s0 s1
+  | _, _ => false
+  end.
+
 Definition off := int.
 Definition imm := int.
 
@@ -25,10 +66,32 @@ Inductive binOp: Type :=
   BPF_ADD | BPF_SUB | BPF_MUL | BPF_DIV | BPF_OR | BPF_AND
 | BPF_LSH | BPF_RSH | BPF_MOD | BPF_XOR | BPF_MOV| BPF_ARSH.
 
+Lemma binOp_eq: forall (b1 b2: binOp), {b1=b2} + {b1<>b2}.
+Proof.
+  decide equality.
+Defined.
+
+Definition binOp_eqb (b0 b1: binOp): bool :=
+  match b0, b1 with
+  | BPF_ADD, BPF_ADD
+  | BPF_SUB, BPF_SUB
+  | BPF_MUL, BPF_MUL
+  | BPF_DIV, BPF_DIV
+  | BPF_OR,  BPF_OR
+  | BPF_AND, BPF_AND
+  | BPF_LSH, BPF_LSH
+  | BPF_RSH, BPF_RSH
+  | BPF_MOD, BPF_MOD
+  | BPF_XOR, BPF_XOR
+  | BPF_MOV, BPF_MOV
+  | BPF_ARSH, BPF_ARSH => true
+  | _, _ => false
+  end.
+
 Inductive instruction: Type :=
   (**r ALU64/32*)
   | BPF_NEG    : arch -> reg -> instruction
-  | BPF_BINARY : arch -> binOp -> reg -> reg+imm -> instruction  
+  | BPF_BINARY : arch -> binOp -> reg -> reg+imm -> instruction
   (**r Branch *)
   | BPF_JA  : off -> instruction
   | BPF_JUMP: cond -> reg -> reg+imm -> off -> instruction
@@ -43,3 +106,30 @@ Inductive instruction: Type :=
   | BPF_RET  : instruction
   | BPF_ERR  : instruction
 .
+
+Definition bpf_instruction_eqb (a b: instruction) : bool :=
+  match a, b with
+  | BPF_NEG a0 r0, BPF_NEG a1 r1 => arch_eqb a0 a1 && reg_eqb r0 r1
+  | BPF_BINARY a0 b0 r0 ri0, BPF_BINARY a1 b1 r1 ri1 => arch_eqb a0 a1 && binOp_eqb b0 b1 && reg_eqb r0 r1 &&
+      match ri0, ri1 with
+      | inl r0', inl r1' => reg_eqb r0' r1'
+      | inr i0', inr i1' => Int.eq  i0' i1'
+      | _, _ => false
+      end
+  | BPF_JA ofs0, BPF_JA ofs1 => Int.eq ofs0 ofs1
+  | BPF_JUMP c0 r0 ri0 ofs0, BPF_JUMP c1 r1 ri1 ofs1 => cond_eqb c0 c1 && reg_eqb r0 r1 && (match ri0, ri1 with
+      | inl r0', inl r1' => reg_eqb r0' r1'
+      | inr i0', inr i1' => Int.eq  i0' i1'
+      | _, _ => false
+      end) && Int.eq ofs0 ofs1
+  | BPF_LDDW r0 i0, BPF_LDDW r1 i1 => reg_eqb r0 r1 && Int.eq i0 i1
+  | BPF_LDX mc0 d0 s0 ofs0, BPF_LDX mc1 d1 s1 ofs1 => chunk_eqb mc0 mc1 && reg_eqb d0 d1 && reg_eqb s0 s1 && Int.eq ofs0 ofs1
+  | BPF_ST mc0 r0 ri0 ofs0, BPF_ST mc1 r1 ri1 ofs1 => chunk_eqb mc0 mc1 && reg_eqb r0 r1 && (match ri0, ri1 with
+      | inl r0', inl r1' => reg_eqb r0' r1'
+      | inr i0', inr i1' => Int.eq  i0' i1'
+      | _, _ => false
+      end) && Int.eq ofs0 ofs1
+  | BPF_RET, BPF_RET
+  | BPF_ERR, BPF_ERR => true
+  | _, _ => false
+  end.
