proof/CorrectRel.v
@@ -135,8 +135,8 @@ Definition MyListType_correct (b:block) (len: nat) (l: MyListType) (v: val) (stm
         Mem.loadv Mint64 m (Vptr b (Ptrofs.repr (8 * (Z.of_nat pc)))) = Some (Vlong vl)
 .
 
-Definition pc_correct (len: nat) (x: int) (v: val) :=
-  Vint x = v /\  0 <= Int.signed x < Z.of_nat len /\ 0 <= 8 * Z.of_nat len <= Ptrofs.max_unsigned. (**r the number of input instructions should be less than Ptrofs.max_unsigned *)
+Definition pc_correct (x: nat) (v: val) (st: State.state) (m:Memory.Mem.mem) :=
+  Vint (Int.repr (Z.of_nat x)) = v /\  0 <= Z.of_nat x < Z.of_nat (mrs_num st) /\ 0 <= 8 * Z.of_nat (mrs_num st) <= Ptrofs.max_unsigned. (**r the number of input instructions should be less than Ptrofs.max_unsigned *)
 
 
 Definition len_correct (len: nat) (x: int) (v: val) :=
