comm/LemmaNat.v
@@ -1,0 +1,176 @@
+From compcert Require Import Zbits.
+From Coq Require Import Lia ZArith.
+
+(**r Implemented by FB
+  a set of useful lemmas about Nat.land
+ *)
+
+Open Scope Z_scope.
+
+Fixpoint Forall_exec (P : nat -> bool) (n: nat)  : bool :=
+  match n with
+  | O => P O
+  | S n' => P n && Forall_exec P n'
+  end.
+
+Lemma Forall_exec_spec : forall P b,
+    Forall_exec P b = true ->
+    forall n, (n <= b)%nat -> P n = true.
+Proof.
+  induction b.
+  - simpl. intros.
+    assert (n=0%nat) by lia.
+    subst. auto.
+  - simpl. intros.
+    rewrite Bool.andb_true_iff in H.
+    assert ( n <= b \/ n = S b)%nat by lia.
+    destruct H1 ; subst.
+    apply IHb; auto. tauto.
+    tauto.
+Qed.
+
+Lemma odd_of_nat : forall (n:nat), Z.odd (Z.of_nat n) = Nat.odd n.
+Proof.
+  intros.
+  destruct (Nat.odd n) eqn:NO.
+  - rewrite Nat.odd_spec in NO.
+    unfold Nat.Odd in NO.
+    destruct NO.
+    subst.
+    rewrite Nat2Z.inj_add.
+    rewrite Nat2Z.inj_mul.
+    rewrite Z.add_comm.
+    rewrite Z.odd_add_mul_2.
+    reflexivity.
+  - destruct (Z.odd (Z.of_nat n)) eqn:ZO; auto.
+    rewrite Z.odd_spec in ZO.
+    destruct ZO.
+    assert (exists m, n = 1 + 2 * m)%nat.
+    exists (Z.to_nat x). lia.
+    destruct H0.
+    subst.
+    rewrite Nat.odd_add_mul_2 in NO.
+    discriminate.
+Qed.
+
+Lemma testbit_of_nat : forall m n,
+  Z.testbit (Z.of_nat n) (Z.of_nat m) = Nat.testbit n m.
+Proof.
+  induction m.
+  - intros.
+    simpl. apply odd_of_nat.
+  - rewrite Nat2Z.inj_succ.
+    simpl. intro.
+    rewrite <- IHm.
+    rewrite Ztestbit_succ by lia.
+    f_equal.
+    rewrite Nat.div2_div.
+    rewrite div_Zdiv by lia.
+    lia.
+Qed.
+
+Lemma testbit_of_nat_ext : forall i n,
+    Z.testbit (Z.of_nat n) i = if Z.leb 0 i
+                               then Nat.testbit n (Z.to_nat i)
+                               else false.
+Proof.
+  intros.
+  destruct (0 <=? i) eqn:LE.
+  -
+    apply Zle_bool_imp_le  in LE.
+    assert (exists m, Z.of_nat m = i).
+    {
+      exists (Z.to_nat i).
+      lia.
+    }
+    destruct H as (m & EQ).
+    rewrite <- EQ.
+    assert (Z.to_nat (Z.of_nat m) = m) by lia.
+    rewrite H.
+    apply testbit_of_nat.
+  - assert (i < 0) by lia.
+    destruct i.
+    + lia.
+    + lia.
+    + reflexivity.
+Qed.
+
+Lemma land_land : forall n m,
+    Z.land (Z.of_nat n) (Z.of_nat m) = Z.of_nat (Nat.land n m).
+Proof.
+  intros.
+  apply Z.bits_inj.
+  unfold Z.eqf.
+  intros.
+  rewrite testbit_of_nat_ext.
+  destruct (0 <=? n0) eqn:NO.
+  assert (exists i, n0 = Z.of_nat i).
+  {
+    exists (Z.to_nat n0).
+    lia.
+  }
+  destruct H. subst.
+  assert (Z.to_nat (Z.of_nat x) = x) by lia.
+  rewrite  H.
+  rewrite Z.land_spec.
+  rewrite Nat.land_spec.
+  rewrite !testbit_of_nat. (**r ? (without natural) performs the rewrite as many times as possible (possibly zero times). This form never fails. ! (without natural) performs the rewrite as many times as possible and at least once. The tactic fails if the requested number of rewrites can't be performed. *)
+  reflexivity.
+  rewrite Z.land_spec.
+  rewrite! testbit_of_nat_ext.
+  destruct(0 <=? n0) ; try congruence.
+  reflexivity.
+Qed.
+
+Close Scope Z_scope.
+
+Lemma land_bound : forall n x, Nat.land n x <= n.
+Proof.
+  unfold Nat.land.
+  intros n x.
+  assert (forall n a b, a <= n -> Nat.bitwise andb n a b <= a).
+  {
+    clear.
+    induction n.
+    - simpl. lia.
+    - intros.
+      simpl.
+      assert (Nat.bitwise andb n (Nat.div2 a) (Nat.div2 b) <= (Nat.div2 a)).
+      {
+        apply IHn.
+        apply Nat.div2_decr.
+        auto.
+      }
+      revert H0.
+      generalize (Nat.bitwise andb n (Nat.div2 a) (Nat.div2 b)) as n1.
+      intros.
+      rewrite Nat.div2_div in H0.
+      rewrite (Nat.div_mod a 2) at 2 by lia.
+      assert (a mod 2 = if Nat.odd a then 1 else 0).
+      {
+        destruct (Nat.odd a) eqn:O.
+        apply Nat.odd_spec in O.
+        unfold Nat.Odd in O.
+        destruct O as (m & E).
+        subst.
+        replace (2 * m + 1) with (1 + m * 2) by lia.
+        rewrite Nat.mod_add. reflexivity.
+        lia.
+        assert (negb (Nat.odd a) = true).
+        { rewrite O; reflexivity. }
+        rewrite Nat.negb_odd in H1.
+        rewrite Nat.even_spec in H1.
+        destruct H1 as (x & EQ).
+        subst.
+        rewrite mult_comm.
+        rewrite Nat.mod_mul. reflexivity. lia.
+      }
+      destruct  (Nat.odd a).
+      rewrite H1.
+      unfold andb.
+      destruct (Nat.odd b) ; lia.
+      unfold andb. lia.
+  }
+  apply H.
+  lia.
+Qed.
