comm/rBPFAST.v
@@ -19,3 +19,18 @@ Definition memory_chunk_to_valu32 (chunk: memory_chunk): val :=
 
 Definition memory_chunk_to_valu32_upbound (chunk: memory_chunk): val :=
   Vint (Int.repr (Int.max_unsigned-(well_chunk_Z chunk))).
+
+Definition chunk_eqb (c1 c2: memory_chunk) : bool :=
+  match c1, c2 with
+  | Mint8signed, Mint8signed
+  | Mint8unsigned, Mint8unsigned
+  | Mint16signed, Mint16signed
+  | Mint16unsigned, Mint16unsigned
+  | Mint32, Mint32
+  | Mint64, Mint64
+  | Mfloat32, Mfloat32
+  | Mfloat64, Mfloat64
+  | Many32, Many32
+  | Many64, Many64 => true
+  | _, _ => false
+  end.
