simulation/correct_get_mem_region.v
@@ -1,0 +1,94 @@
+From Coq Require Import List ZArith.
+Import ListNotations.
+From dx Require Import ResultMonad IR.
+From bpf.comm Require Import MemRegion Regs State Monad rBPFAST rBPFValues.
+From bpf.monadicmodel Require Import rBPFInterpreter.
+
+From compcert Require Import Coqlib Values Clight Memory Integers.
+
+From bpf.clight Require Import interpreter.
+
+From bpf.proof Require Import MatchState Clightlogic clight_exec CommonLemma CorrectRel.
+
+(*
+Check get_mem_region.
+
+get_mem_region
+     : nat -> MyMemRegionsType -> M memory_region *)
+
+Section Get_mem_region.
+
+  (** The program contains our function of interest [fn] *)
+  Definition p : Clight.program := prog.
+
+  (* [Args,Res] provides the mapping between the Coq and the C types *)
+  Definition args : list Type := [(nat:Type); (list memory_region:Type)].
+  Definition res : Type := (memory_region:Type).
+
+  (* [f] is a Coq Monadic function with the right type *)
+  Definition f : arrow_type args (M res) := get_mem_region.
+
+  Variable state_block: block. (**r a block storing all rbpf state information? *)
+  Variable mrs_block: block.
+  Variable ins_block: block.
+
+  (* [fn] is the Cligth function which has the same behaviour as [f] *)
+  Definition fn: Clight.function := f_get_mem_region.
+
+  Definition stateM_correct (st:unit) (v: val) (stm:State.state) (m: Memory.Mem.mem) :=
+    v = Vptr state_block Ptrofs.zero /\ match_state state_block mrs_block ins_block stm m.
+
+  (* [match_arg] relates the Coq arguments and the C arguments *)
+  Definition match_arg_list : DList.t (fun x => x -> val -> State.state -> Memory.Mem.mem -> Prop) args :=
+      (DList.DCons pc_correct
+        (DList.DCons (match_region_list mrs_block)
+                (DList.DNil _))).
+
+  (* [match_res] relates the Coq result and the C result *)
+  Definition match_res : res -> val -> State.state -> Memory.Mem.mem -> Prop := fun r v st m => List.In r (bpf_mrs st).
+
+  Instance correct_function3_get_mem_region : forall a, correct_function3 p args res f fn (nil) true match_arg_list match_res a.
+  Proof.
+    correct_function_from_body args.
+    correct_body.
+    (** how to use correct_* *)
+    unfold INV.
+    unfold f.
+    repeat intro.
+    get_invariant _n.
+    get_invariant _mrs.
+
+    unfold pc_correct in c1.
+    destruct c1 as (Hv_eq & Hrange & Hmax).
+    unfold match_region_list in c2.
+    destruct c2 as (Hv0_eq & Hmrs_eq & Hmrs_num_eq & Hmatch).
+    subst.
+
+    eexists; exists m, Events.E0.
+    split.
+    {
+      repeat forward_star.
+    }
+    split.
+    {
+      unfold match_res, match_res, MyMemRegionsIndexnat, Memory_regions.index_nat.
+      apply nth_error_In with (n:= c).
+      assert (Hlen: (c < List.length (bpf_mrs st))%nat). {
+        rewrite Hmrs_num_eq.
+        lia.
+      }
+      apply nth_error_nth' with (d:= default_memory_region) in Hlen.
+      rewrite Hlen.
+      unfold res.
+      rewrite Hlen.
+      reflexivity.
+    }
+    split.
+    constructor.
+    simpl; split; reflexivity.
+Qed.
+
+End Get_mem_region.
+
+Existing Instance correct_function3_get_mem_region.
+
